Mostly-complete concurrent queue example.

progs/verif_ghost_queue.v
@@ -1,9 +1,10 @@
-Require Import progs.verif_cond_queue.
-Require Import progs.verif_incr.
-Require Import msl.predicates_sl.
-Require Import floyd.proofauto.
+Require Import progs.conclib.
 Require Import concurrency.semax_conc.
+Require Import floyd.proofauto.
 Require Import progs.ghost_queue.
+Require Import Sorting.Sorted.
+
+Set Bullet Behavior "Strict Subproofs".
 
 Instance CompSpecs : compspecs. make_compspecs prog. Defined.
 Definition Vprog : varspecs. mk_varspecs prog. Defined.
@@ -53,92 +54,107 @@ Parameter Ghost : forall (sh : share) (t : type) (v : reptype t) (p : val), Pred
 Axiom interp_ghost : forall sh t v p, Interp (Ghost sh t v p) = ghost sh t v p.
 Axiom ghost_inj : forall sh1 sh2 t v1 v2 p, ghost sh1 t v1 p * ghost sh2 t v2 p |-- !!(v1 = v2).
 
-(* Note that a writable share must include all readable shares. *)
-Definition lock_pred sh buf len next := Exp _ (fun reqs => Exp _ (fun n => Exp _ (fun n' =>
-  Pred_list (Data_at _ Ews (tarray (tptr trequest) (Z.of_nat MAX)) (complete reqs) buf ::
-             Data_at _ Ews (tarray tint 1) [Vint (Int.repr (Zlength reqs))] len ::
-             Pred_prop (Int.min_signed <= n' <= n /\ n <= Int.max_signed /\ (length reqs <= MAX)%nat) ::
-             Data_at _ Ews (tarray tint 1) [Vint (Int.repr n)] next ::
-             Ghost sh tint (Vint (Int.repr n')) next ::
-             map (fun r => Exp _ (fun data => Pred_list [Pred_prop (data < n);
-               Data_at _ Tsh trequest (Vint (Int.repr data)) r])) reqs)))).
+Definition MAX : nat := 10.
 
-(* We would like the postcondition to tell us that the new request is  smaller than next. But because next is
-   part of a lock invariant, we can only state this when the lock is held! *)
+Definition rotate {A} (l : list A) n m := skipn (m - n) l ++ firstn (m - n) l.
+
+(* Note that a writable share must include all readable shares. *)
+Definition lock_pred' sh buf ends len next ghosts reqs times head tail n ns := Pred_list (
+    Data_at _ Ews (tarray (tptr trequest) (Z.of_nat MAX)) (rotate (complete MAX reqs) head MAX) buf ::
+    Data_at _ Ews (tarray tint 2) [Vint (Int.repr (Z.of_nat head)); Vint (Int.repr (Z.of_nat tail))] ends ::
+    Data_at _ Ews (tarray tint 1) [Vint (Int.repr (Zlength reqs))] len ::
+    Pred_prop (Forall (fun d => Int.min_signed <= d < n /\ Forall (fun n => n < d) ns) times /\
+               Int.min_signed <= n <= Int.max_signed /\ Forall (fun n' => Int.min_signed <= n' < n) ns /\
+               (length reqs <= MAX /\ length times = length reqs /\ length ns = length ghosts)%nat /\
+               Sorted Z.lt times /\
+               (head < MAX)%nat /\ Z.of_nat tail = (Z.of_nat head + Zlength reqs) mod Z.of_nat MAX) ::
+    Data_at _ Ews (tarray tint 1) [Vint (Int.repr n)] next ::
+    map (fun p => Ghost sh tint (Vint (Int.repr (fst p))) (snd p)) (combine ns ghosts) ++
+    map (fun p => Exp _ (fun d => Data_at _ Tsh trequest (d, Vint (Int.repr (fst p))) (snd p))) (combine times reqs)).
+
+Definition lock_pred sh buf ends len next ghosts := Exp _ (fun reqs => Exp _ (fun times =>
+  Exp _ (fun head => Exp _ (fun tail => Exp _ (fun n => Exp _ (fun ns =>
+  lock_pred' sh buf ends len next ghosts reqs times head tail n ns)))))).
+
 Definition get_request_spec :=
  DECLARE _get_request
-  WITH sh : share, n : Z, lock : val, buf : val, len : val, next : val, gsh1 : share, gsh2 : share
-  PRE [ ]
-    PROP (readable_share sh; Int.min_signed <= n < Int.max_signed; sepalg.join gsh1 gsh2 Ews)
-    LOCAL (gvar _requests_lock lock; gvar _next next)
-    SEP (lock_inv sh lock (Interp (lock_pred gsh2 buf len next)); ghost gsh1 tint (Vint (Int.repr n)) next)
+  WITH _ : unit
+  PRE [ ] PROP () LOCAL () SEP ()
   POST [ tptr trequest ]
-    EX n' : Z, EX v : val, EX data : Z,
-    PROP (data < n')
+    EX v : val, EX d : val, EX t : val,
+    PROP ()
     LOCAL (temp ret_temp v)
-    SEP (lock_inv sh lock (Interp (lock_pred gsh2 buf len next));
-         ghost gsh1 tint (Vint (Int.repr n')) next;
-         data_at Tsh trequest (Vint (Int.repr data)) v).
+    SEP (data_at Tsh trequest (d, t) v).
 
 Definition process_request_spec :=
  DECLARE _process_request
-  WITH request : val, data : Z
+  WITH request : val, d : val, t : Z
   PRE [ _request OF (tptr trequest) ]
      PROP ()
      LOCAL (temp _request request)
-     SEP (data_at Tsh trequest (Vint (Int.repr data)) request)
+     SEP (data_at Tsh trequest (d, Vint (Int.repr t)) request)
   POST [ tint ]
-    PROP () LOCAL (temp ret_temp (Vint (Int.repr data))) SEP (emp).
+    PROP () LOCAL (temp ret_temp (Vint (Int.repr t))) SEP (emp).
+
+Notation "'WITH'  x1 : t1 , x2 : t2 , x3 : t3 , x4 : t4 , x5 : t5 , x6 : t6 , x7 : t7 , x8 : t8 , x9 : t9 , x10 : t10 , x11 : t11 , x12 : t12 , x13 : t13 , x14 : t14 , x15 : t15 'PRE'  [ u , .. , v ] P 'POST' [ tz ] Q" :=
+     (mk_funspec ((cons u%formals .. (cons v%formals nil) ..), tz) cc_default (t1*t2*t3*t4*t5*t6*t7*t8*t9*t10*t11*t12*t13*t14*t15)
+           (fun x => match x with (x1,x2,x3,x4,x5,x6,x7,x8,x9,x10,x11,x12,x13,x14,x15) => P%assert end)
+           (fun x => match x with (x1,x2,x3,x4,x5,x6,x7,x8,x9,x10,x11,x12,x13,x14,x15) => Q%assert end))
+            (at level 200, x1 at level 0, x2 at level 0, x3 at level 0, x4 at level 0, 
+             x5 at level 0, x6 at level 0, x7 at level 0, x8 at level 0, x9 at level 0,
+              x10 at level 0, x11 at level 0, x12 at level 0,  x13 at level 0, x14 at level 0, x15 at level 0,
+             P at level 100, Q at level 100).
 
 Definition add_spec :=
  DECLARE _add
-  WITH sh : share, n : Z, lock : val, request : val, data : Z, buf : val, len : val, next : val,
-       cprod : val, ccon : val, gsh1 : share, gsh2 : share
+  WITH sh : share, lock : val, request : val, d : val, t : val, buf : val, ends : val, len : val, next : val,
+       cprod : val, ccon : val, ghosts : list val, gsh2 : share
   PRE [ _request OF (tptr trequest) ]
-   PROP (readable_share sh; Int.min_signed <= n <= Int.max_signed; data < n)
-   LOCAL (temp _request request; gvar _buf buf; gvar _length len; gvar _requests_lock lock;
-          gvar _requests_producer cprod; gvar _requests_consumer ccon)
-   SEP (lock_inv sh lock (Interp (lock_pred gsh2 buf len next)); cond_var sh cprod; cond_var sh ccon;
-        data_at Tsh trequest (Vint (Int.repr data)) request; ghost gsh1 tint (Vint (Int.repr n)) next)
+   PROP (readable_share sh)
+   LOCAL (temp _request request; gvar _buf buf; gvar _ends ends; gvar _length len; gvar _next next;
+          gvar _requests_lock lock; gvar _requests_producer cprod; gvar _requests_consumer ccon)
+   SEP (lock_inv sh lock (Interp (lock_pred gsh2 buf ends len next ghosts)); cond_var sh cprod; cond_var sh ccon;
+        data_at Tsh trequest (d, t) request)
   POST [ tvoid ]
-   EX n' : Z, PROP () LOCAL ()
-   SEP (lock_inv sh lock (Interp (lock_pred gsh2 buf len next)); cond_var sh cprod; cond_var sh ccon;
-        ghost gsh1 tint (Vint (Int.repr n')) next).
-(* Here's where we might need ghost variables to record the nature of the change? *)
+   PROP () LOCAL ()
+   SEP (lock_inv sh lock (Interp (lock_pred gsh2 buf ends len next ghosts)); cond_var sh cprod; cond_var sh ccon).
 
 Definition remove_spec :=
  DECLARE _remove
-  WITH sh : share, n : Z, lock : val, buf : val, len : val, next : val, cprod : val, ccon : val,
-       gsh1 : share, gsh2 : share
+  WITH sh : share, t : Z, lock : val, buf : val, ends : val, len : val, next : val, cprod : val, ccon : val,
+       ghosts : list val, i : nat, g : val, gsh1 : share, gsh2 : share
   PRE [ ]
-   PROP (readable_share sh; Int.min_signed <= n < Int.max_signed; sepalg.join gsh1 gsh2 Ews)
-   LOCAL (gvar _buf buf; gvar _length len; gvar _requests_lock lock; gvar _requests_producer cprod;
-          gvar _requests_consumer ccon)
-   SEP (lock_inv sh lock (Interp (lock_pred gsh2 buf len next)); cond_var sh cprod; cond_var sh ccon;
-        ghost gsh1 tint (Vint (Int.repr n)) next)
+   PROP (readable_share sh; Int.min_signed <= t <= Int.max_signed; sepalg.join gsh1 gsh2 Ews;
+         nth_error ghosts i = Some g)
+   LOCAL (gvar _buf buf; gvar _ends ends; gvar _length len; gvar _requests_lock lock;
+          gvar _requests_producer cprod; gvar _requests_consumer ccon)
+   SEP (lock_inv sh lock (Interp (lock_pred gsh2 buf ends len next ghosts)); cond_var sh cprod; cond_var sh ccon;
+        ghost gsh1 tint (Vint (Int.repr t)) g)
   POST [ tptr trequest ]
-   EX n' : Z, EX req : val, EX data : Z,
-   PROP (data < n')
+   EX t' : Z, EX req : val, EX d : val,
+   PROP (t < t' <= Int.max_signed)
    LOCAL (temp ret_temp req)
-   SEP (lock_inv sh lock (Interp (lock_pred gsh2 buf len next)); cond_var sh cprod; cond_var sh ccon;
-        data_at Tsh trequest (Vint (Int.repr data)) req; ghost gsh1 tint (Vint (Int.repr n')) next).
+   SEP (lock_inv sh lock (Interp (lock_pred gsh2 buf ends len next ghosts)); cond_var sh cprod; cond_var sh ccon;
+        data_at Tsh trequest (d, Vint (Int.repr t')) req; ghost gsh1 tint (Vint (Int.repr t')) g).
 
-Definition t_lock_pred := Pred_list [].
+Definition t_lock_pred sh cprod ccon lock lockt buf ends len next ghosts gsh1 gsh2 g :=
+  Self_lock (Pred_list [Cond_var _ sh cprod; Cond_var _ sh ccon;
+    Lock_inv sh lock (lock_pred gsh2 buf ends len next ghosts);
+    Exp _ (fun n => Ghost gsh1 tint (Vint (Int.repr n)) g)]) sh lockt.
 
 Definition f_spec :=
  DECLARE _f
-  WITH sh : share, lock : val, wsh : share, buf : val, len : val, next : val, lockt : val
+  WITH sh : share, t : Z, lock : val, buf : val, ends : val, len : val, next : val, lockt : val,
+       cprod : val, ccon : val, ghosts : list val, i : nat, g : val, gsh1 : share, gsh2 : share
   PRE [ _arg OF (tptr tvoid) ]
-   PROP ()
-   LOCAL (gvar _buf buf; gvar _length len; gvar _requests_lock lock; temp _arg lockt)
-   SEP (lock_inv sh lock (Interp (lock_pred wsh buf len next)); lock_inv sh lockt (Interp (t_lock_pred)))
-  POST [ tvoid ]
-   EX last : Z, EX res : val, EX v1 : Z, EX v2 : Z, EX v3 : Z,
-   PROP (last < v1; v1 < v2; v2 < v3)
-   LOCAL (temp _last (Vint (Int.repr last)); temp _res res)
-   SEP (lock_inv sh lock (Interp (lock_pred wsh buf len next));
-        lock_inv sh lockt (Interp (t_lock_pred));
-        data_at Tsh (tarray tint 3) [Vint (Int.repr v1); Vint (Int.repr v2); Vint (Int.repr v3)] res).
+   PROP (readable_share sh; Int.min_signed <= t <= Int.max_signed; sepalg.join gsh1 gsh2 Ews;
+         nth_error ghosts i = Some g)
+   LOCAL (gvar _buf buf; gvar _ends ends; gvar _length len; gvar _next next; gvar _requests_lock lock;
+          temp _arg lockt; gvar _requests_producer cprod; gvar _requests_consumer ccon)
+   SEP (lock_inv sh lock (Interp (lock_pred gsh2 buf ends len next ghosts));
+        lock_inv sh lockt (Interp (t_lock_pred sh cprod ccon lock lockt buf ends len next ghosts gsh1 gsh2 g));
+        cond_var sh cprod; cond_var sh ccon; ghost gsh1 tint (Vint (Int.repr t)) g)
+  POST [ tptr tvoid ] PROP () LOCAL () SEP (emp).
 
 Definition main_spec :=
  DECLARE _main
@@ -151,17 +167,8 @@ Definition Gprog : funspecs := augment_funspecs prog [acquire_spec; release_spec
   malloc_spec; free_spec; get_request_spec; process_request_spec; add_spec; remove_spec; f_spec;
   main_spec].
 
-Lemma lt_plus_one : forall n reqs, fold_right sepcon emp (map Interp (map (fun r => Exp _ (fun data =>
-  Pred_list [Pred_prop (data < n); Data_at CompSpecs Tsh trequest (Vint (Int.repr data)) r])) reqs))
-|-- fold_right sepcon emp (map Interp (map (fun r => Exp _ (fun data =>
-  Pred_list [Pred_prop (data < n + 1); Data_at CompSpecs Tsh trequest (Vint (Int.repr data)) r])) reqs)).
-Proof.
-  induction reqs; simpl; entailer!.
-  Exists x; entailer'; cancel.
-Qed.
-
-Lemma inv_precise : forall wsh buf len next (Hbuf : isptr buf) (Hlen : isptr len) (Hnext : isptr next),
-  precise (Interp (lock_pred wsh buf len next)).
+Lemma inv_precise : forall gsh2 buf ends len next ghosts (Hbuf : isptr buf) (Hlen : isptr len) (Hnext : isptr next),
+  precise (Interp (lock_pred gsh2 buf ends len next ghosts)).
 Proof.
   simpl.
 (*  intros; apply derives_precise with (Q := data_at_ Tsh (tarray (tptr trequest) 10) buf *
@@ -189,8 +196,8 @@ Proof.
     apply precise_emp.*)
 Admitted.
 
-Lemma inv_positive : forall wsh buf len next,
-  positive_mpred (Interp (lock_pred wsh buf len next)).
+Lemma inv_positive : forall gsh2 buf ends len next ghosts,
+  positive_mpred (Interp (lock_pred gsh2 buf ends len next ghosts)).
 Proof.
 Admitted.
 
@@ -218,6 +225,48 @@ Proof.
   intro X; rewrite <- (Int.signed_repr n1), <- (Int.signed_repr n2); congruence.
 Qed.*)
 
+Lemma nth_ghost : forall sh i ns ghosts g (Hlen : length ns = length ghosts)
+  (Hg : nth_error ghosts i = Some g), exists n, nth_error ns i = Some n /\
+  fold_right sepcon emp (map Interp (map (fun p => Ghost sh tint (Vint (Int.repr (fst p))) (snd p))
+    (combine ns ghosts))) =
+  fold_right sepcon emp (map Interp (map (fun p => Ghost sh tint (Vint (Int.repr (fst p))) (snd p))
+    (combine (remove_at i ns) (remove_at i ghosts)))) * ghost sh tint (Vint (Int.repr n)) g.
+Proof.
+  induction i; simpl; intros.
+  - destruct ghosts; inv Hg.
+    destruct ns; [discriminate|].
+    eexists; split; eauto; unfold remove_at; simpl.
+    rewrite interp_ghost, sepcon_comm; auto.
+  - destruct ghosts; [discriminate|].
+    destruct ns; [discriminate|].
+    inversion Hlen as [Hlen'].
+    specialize (IHi _ _ _ Hlen' Hg); destruct IHi as (n & Hn & Heq).
+    exists n; split; auto; unfold remove_at; simpl.
+    rewrite Heq, sepcon_assoc; auto.
+Qed.
+
+Lemma add_nth_ghost : forall sh i ns ghosts g n (Hlen : length ns = length ghosts)
+  (Hg : nth_error ghosts i = Some g),
+  fold_right sepcon emp (map Interp (map (fun p => Ghost sh tint (Vint (Int.repr (fst p))) (snd p))
+    (combine (remove_at i ns) (remove_at i ghosts)))) * ghost sh tint (Vint (Int.repr n)) g =
+  fold_right sepcon emp (map Interp (map (fun p => Ghost sh tint (Vint (Int.repr (fst p))) (snd p))
+    (combine (upd_Znth (Z.of_nat i) ns n) ghosts))).
+Proof.
+  induction i; intros.
+  - destruct ghosts; inv Hg.
+    destruct ns; [discriminate|].
+    unfold remove_at; simpl.
+    rewrite sublist_1_cons, Zlength_cons, sublist_same; auto; [|omega].
+    rewrite interp_ghost, sepcon_comm; auto.
+  - destruct ghosts; [discriminate|].
+    destruct ns; [discriminate|].
+    inversion Hlen as [Hlen'].
+    rewrite Nat2Z.inj_succ, upd_Znth_cons; [|omega].
+    unfold Z.succ; rewrite Z.add_simpl_r.
+    unfold remove_at; simpl.
+    rewrite sepcon_assoc; setoid_rewrite IHi; auto.
+Qed.
+
 Lemma body_get_request : semax_body Vprog Gprog f_get_request get_request_spec.
 Proof.
   start_function.
@@ -229,47 +278,14 @@ Proof.
   unfold malloc_compatible in *.
   destruct p; try contradiction; match goal with H : _ /\ _ |- _ => destruct H end.
   rewrite memory_block_data_at_.
-  forward_call (lock, sh, lock_pred gsh2 buf len next).
-  simpl; Intros reqs n1 n2.
   forward.
   forward.
-  forward.
-  unfold upd_Znth, Znth; simpl.
-  rewrite sublist.sublist_nil; simpl.
-  rewrite add_repr.
-  rewrite data_at_isptr, (data_at_isptr _ (tarray tint 1)), field_at_isptr; normalize.
-  forward_call (lock, sh, lock_pred gsh2 buf len next).
-  { simpl; Exists reqs (n1 + 1) (n1 + 1).
-    unfold fold_right at 2; cancel.
-    repeat rewrite interp_ghost.
-    rewrite sepcon_comm.
-    rewrite <- sepcon_assoc.
-    rewrite (sepcon_comm _ (ghost _ _ _ _)).
-    repeat rewrite <- sepcon_assoc.
-    rewrite sepcon_assoc.
-    eapply derives_trans; [apply sepcon_derives; [apply prop_and_same_derives, ghost_inj | apply derives_refl]|].
-    normalize.
-    assert (n2 = n).
-    { rewrite <- (Int.signed_repr n2), <- (Int.signed_repr n); try omega; congruence. }
-    subst; apply andp_right; [apply prop_right; repeat split; auto; try omega|].
-    { admit. } (* Here's where we need better handling for max_signed. *)
-    erewrite ghost_join; eauto.
-    rewrite sepcon_assoc; eapply derives_trans; [eapply sepcon_derives; [|apply derives_refl]|].
-    { apply change_ghost with (v' := Vint (Int.repr (n1 + 1))). }
-    erewrite <- ghost_join; eauto; cancel.
-    rewrite sepcon_assoc, sepcon_comm, sepcon_assoc.
-    apply sepcon_derives; [apply lt_plus_one | cancel]. }
-  { split; auto; split; [apply inv_precise | apply inv_positive]; auto. }
-  eapply semax_pre; [|apply semax_return].
-  subst POSTCONDITION; unfold abbreviate.
-  go_lower; ent_iter.
-  Exists (n1 + 1) (Vptr b i) n1; entailer'; cancel.
+  Exists (Vptr b i0) (Vint (Int.repr 1)) Vundef; entailer.
   { unfold field_compatible; simpl; repeat split; auto.
     unfold align_attr; simpl.
     simpl in *.
     eapply Zdivides_trans; eauto; unfold natural_alignment; exists 2; omega. }
-Admitted.
-(* We should actually do something smart when we hit max_signed, so we don't run out. *)
+Qed.
 
 Lemma body_process_request : semax_body Vprog Gprog f_process_request process_request_spec.
 Proof.
@@ -281,206 +297,368 @@ Proof.
   forward.
 Qed.
 
-Lemma derives_refl' : forall Delta P Q R, ENTAIL Delta, PROPx (P) (LOCALx (Q) (SEPx (R))) |--
-  PROPx (P) (LOCALx (Q) (SEPx (R))).
+Lemma mods_repr : forall a b, 0 <= a <= Int.max_signed -> 0 < b <= Int.max_signed ->
+  Int.mods (Int.repr a) (Int.repr b) = Int.repr (a mod b).
 Proof.
-  go_lowerx; entailer'.
+  intros.
+  unfold Int.mods.
+  pose proof Int.min_signed_neg.
+  rewrite Zquot.Zrem_Zmod_pos; repeat rewrite Int.signed_repr; auto; omega.
+Qed.
+
+Lemma upd_rotate : forall {A} i (l : list A) n m x (Hl : length l = m) (Hlt : (n < m)%nat)
+  (Hi : 0 <= i < Z.of_nat (length l)),
+  upd_Znth i (rotate l n m) x = rotate (upd_Znth ((i - Z.of_nat n) mod Z.of_nat m) l x) n m.
+Proof.
+  intros; unfold upd_Znth, rotate.
+  repeat rewrite sublist_firstn.
+  assert (length (skipn (m - n) l) = n).
+  { rewrite skipn_length; omega. }
+  assert (Zlength (skipn (m - n) l ++ firstn (m - n) l) = Zlength l) as Hl'.
+  { repeat rewrite Zlength_correct.
+    rewrite app_length, skipn_length, firstn_length, Min.min_l; Omega0. }
+  destruct (Z_lt_dec i (Z.of_nat n)).
+  - replace ((i - Z.of_nat n) mod Z.of_nat m) with (Z.of_nat (m + Z.to_nat i - n))%nat.
+    rewrite Nat2Z.id.
+    rewrite firstn_app1; [|Omega0].
+    assert (m - n <= Datatypes.length (firstn (m + Z.to_nat i - n) l))%nat.
+    { rewrite firstn_length, Min.min_l; Omega0. }
+    rewrite skipn_app1; auto.
+    rewrite skipn_firstn.
+    rewrite firstn_app1, firstn_firstn; auto; try omega.
+    replace (m + Z.to_nat i - n - (m - n))%nat with (Z.to_nat i); [|omega].
+    rewrite <- app_assoc; f_equal.
+    simpl; f_equal.
+    rewrite Hl', sublist.sublist_app; try (rewrite Zlength_correct; omega).
+    assert (Zlength (skipn (m - n) l) = Z.of_nat n) as Hm' by (rewrite Zlength_correct; omega).
+    repeat rewrite Hm'.
+    rewrite Z.min_l; [|omega].
+    rewrite Z.min_r; [|rewrite Zlength_correct; omega].
+    rewrite Z.max_r; [|omega].
+    rewrite sublist_firstn.
+    rewrite Z.max_l; [|rewrite Zlength_correct; omega].
+    unfold sublist.sublist.
+    rewrite skipn_skipn.
+    replace (Zlength l - (Z.of_nat (m + Z.to_nat i - n) + 1)) with (Z.of_nat n - (i + 1)).
+    repeat rewrite Z2Nat.inj_add; try omega.
+    rewrite Nat2Z.id.
+    replace (m - _ + _)%nat with (m + Z.to_nat i - n + Z.to_nat 1)%nat by omega.
+    f_equal.
+    replace (Z.to_nat (Zlength l - Z.of_nat n)) with (m - n)%nat by (rewrite Zlength_correct; Omega0).
+    rewrite firstn_firstn; auto.
+    { rewrite Zlength_correct, Nat2Z.inj_sub, Nat2Z.inj_add, Z2Nat.id; omega. }
+    { rewrite <- Hl', Zlength_app; omega. }
+    { rewrite Zmod_eq; [|omega].
+      replace (_ / _) with (-1); try Omega0.
+      replace (_ - _) with (- (Z.of_nat n - i)); [|omega].
+      rewrite Z_div_nz_opp_full, Zdiv_small; try omega.
+      rewrite Zmod_small; omega. }
+  - assert (n <= Z.to_nat i)%nat.
+    { rewrite Nat2Z.inj_le, Z2Nat.id; omega. }
+    rewrite firstn_app2; rewrite H; auto.
+    destruct Hi as (? & Hi).
+    assert (Z.to_nat i < length l)%nat.
+    { rewrite Z2Nat.inj_lt, Nat2Z.id in Hi; omega. }
+    assert (Z.to_nat i - n <= m - n)%nat by omega.
+    rewrite firstn_firstn; auto.
+    rewrite Zmod_small; [|omega].
+    assert (length (firstn (Z.to_nat (i - Z.of_nat n)) l) = Z.to_nat (i - Z.of_nat n)) as Hl1.
+    { rewrite firstn_length, Min.min_l; auto.
+      rewrite Z2Nat.inj_sub, Nat2Z.id; omega. }
+    assert (m - n >= Z.to_nat (i - Z.of_nat n))%nat.
+    { rewrite Z2Nat.inj_sub, Nat2Z.id; omega. }
+    rewrite skipn_app2; rewrite Hl1; auto.
+    assert (m - n - Z.to_nat (i - Z.of_nat n) = m - Z.to_nat i)%nat as Hminus.
+    { rewrite Z2Nat.inj_sub; [|omega].
+      rewrite <- NPeano.Nat.sub_add_distr, Nat2Z.id, le_plus_minus_r; omega. }
+    rewrite Hminus.
+    destruct (m - Z.to_nat i)%nat eqn: Hi'; [omega | simpl].
+    rewrite firstn_app2; rewrite Hl1; auto.
+    rewrite Hminus; clear Hminus; simpl.
+    unfold sublist.sublist at 2.
+    rewrite skipn_firstn, skipn_skipn.
+    assert (Z.to_nat (i - Z.of_nat n + 1) + n1 = m - n)%nat as Hminus'.
+    { assert (m - Z.to_nat i + Z.to_nat i = S n1 + Z.to_nat i)%nat as Heq by (f_equal; auto).
+      rewrite NPeano.Nat.sub_add in Heq; [|omega].
+      rewrite Heq.
+      rewrite Z2Nat.inj_add, Z2Nat.inj_sub, Nat2Z.id; simpl Z.to_nat; omega. }
+    rewrite Hminus'.
+    assert (n1 = Z.to_nat (Zlength l - (i + 1)))%nat.
+    { rewrite Z2Nat.inj_sub, Zlength_correct, Nat2Z.id, Z2Nat.inj_add; simpl; omega. }
+    subst n1.
+    replace (Z.to_nat (Zlength l - _) - _)%nat with (length (skipn (m - n) l)).
+    rewrite firstn_exact_length.
+    rewrite <- app_assoc; f_equal.
+    rewrite Z2Nat.inj_sub, Nat2Z.id; [|omega].
+    repeat f_equal.
+    unfold sublist.sublist.
+    rewrite Hl'.
+    assert (length l - (m - n) = n)%nat as Hskip by (subst m; clear - Hlt; omega).
+    rewrite skipn_app2; rewrite skipn_length, Hskip.
+    rewrite firstn_firstn.
+    rewrite skipn_firstn, firstn_firstn.
+    f_equal.
+    replace (Z.to_nat (i + 1) - n)%nat with (Z.to_nat (i - Z.of_nat n + 1))%nat; auto.
+    { clear - H1 H0 n0; rewrite Z2Nat.inj_add, Z2Nat.inj_sub; try omega.
+      rewrite Nat2Z.id, Z2Nat.inj_add; omega. }
+    { subst m; clear - H1 H0 n0; rewrite Z2Nat.inj_sub; [|omega].
+      rewrite Zlength_correct, Nat2Z.id, Z2Nat.inj_add; omega. }
+    { subst m; clear - H1 H0 n0; rewrite Z2Nat.inj_sub; try omega.
+      rewrite Zlength_correct, Nat2Z.id; rewrite Z2Nat.inj_sub, Nat2Z.id; try omega.
+      repeat rewrite Z2Nat.inj_add; simpl; try omega.
+      rewrite Z2Nat.inj_sub; omega. }
+    { clear - H1 H0; rewrite Z2Nat.inj_add; omega. }
+    { subst m; clear - H1 H0 n0 Hi; rewrite skipn_length; repeat rewrite Z2Nat.inj_sub; try omega.
+      repeat rewrite Zlength_correct, Nat2Z.id.
+      repeat rewrite Z2Nat.inj_add; try omega.
+      rewrite Z2Nat.inj_sub; try omega.
+      rewrite Nat2Z.id.
+      rewrite <- NPeano.Nat.sub_add_distr, plus_comm, <- Nat.add_sub_swap; [omega | Omega0]. }
+Qed.
+
+Lemma combine_app : forall {A B} (l1 l2 : list A) (l1' l2' : list B), length l1 = length l1' ->
+  combine (l1 ++ l2) (l1' ++ l2') = combine l1 l1' ++ combine l2 l2'.
+Proof.
+  induction l1; destruct l1'; intros; try discriminate; auto; simpl in *.
+  rewrite IHl1; auto.
+Qed.
+
+Lemma length_complete : forall l m, (length l <= m)%nat -> length (complete m l) = m.
+Proof.
+  intros; unfold complete.
+  rewrite app_length, repeat_length; omega.
 Qed.
 
 Lemma body_add : semax_body Vprog Gprog f_add add_spec.
 Proof.
   start_function.
-  forward_call (lock, sh, lock_pred gsh2 buf len next).
-  simpl; Intros reqs n1 n2.
+  forward_call (lock, sh, lock_pred gsh2 buf ends len next ghosts).
+  simpl; Intros reqs times head tail n ns.
   forward.
   unfold Znth; simpl.
-  forward_while (EX reqs : list val, EX n' : Z,
-   PROP (n <= n' <= Int.max_signed /\ (length reqs <= MAX)%nat)
+  forward_while (EX reqs : list val, EX times : list Z, EX head : nat, EX tail : nat, EX n : Z, EX ns : list Z,
+   PROP ()
    LOCAL (temp _len (Vint (Int.repr (Zlength reqs))); temp _request request; 
-     gvar _buf buf; gvar _length len; gvar _requests_lock lock; gvar _requests_producer cprod;
-     gvar _requests_consumer ccon)
-   SEP (lock_inv sh lock (Interp (lock_pred gsh2 buf len next));
-        data_at Ews (tarray (tptr trequest) (Z.of_nat MAX)) (complete reqs) buf;
-        data_at Ews (tarray tint 1) [Vint (Int.repr (Zlength reqs))] len; emp;
-        data_at Ews (tarray tint 1) [Vint (Int.repr n')] next;
-        fold_right sepcon emp (map Interp (map (fun r => Exp _ (fun data0 =>
-          Pred_list [Pred_prop (data0 < n'); Data_at CompSpecs Tsh trequest (Vint (Int.repr data0)) r])) reqs));
-        cond_var sh cprod; cond_var sh ccon; @data_at CompSpecs Tsh trequest (Vint (Int.repr data)) request;
-        ghost gsh1 tint (Vint (Int.repr n)) next * ghost gsh2 tint (Vint (Int.repr n)) next)).
-  { Exists reqs n1; go_lower; entailer'.
-    repeat rewrite interp_ghost.
-    rewrite sepcon_comm.
-    rewrite <- sepcon_assoc.
-    rewrite (sepcon_comm _ (ghost _ _ _ _)).
-    repeat rewrite <- sepcon_assoc.
-    do 7 rewrite sepcon_assoc.
-    eapply derives_trans; [apply sepcon_derives; [apply prop_and_same_derives, ghost_inj | apply derives_refl]|].
-    normalize.
-    assert (n2 = n).
-    { rewrite <- (Int.signed_repr n2), <- (Int.signed_repr n); try omega; congruence. }
-    subst; entailer'; cancel. }
+     gvar _buf buf; gvar _ends ends; gvar _next next; gvar _length len; gvar _requests_lock lock;
+     gvar _requests_producer cprod; gvar _requests_consumer ccon)
+   SEP (lock_inv sh lock (Interp (lock_pred gsh2 buf ends len next ghosts));
+        Interp (lock_pred' gsh2 buf ends len next ghosts reqs times head tail n ns);
+        cond_var sh cprod; cond_var sh ccon; @data_at CompSpecs Tsh trequest (d, t) request)).
+  { Exists reqs times head tail n ns; go_lower.
+    apply andp_right; [apply prop_right; repeat split; auto |
+      apply andp_right; [apply prop_right; repeat split; auto | normalize; cancel]]. }
   { go_lower; entailer'. }
-  { match goal with H : _ /\ _ |- _ => destruct H end.
-    forward_call (cprod, lock, sh, sh, lock_pred gsh2 buf len next).
-    { simpl; cancel.
-      Exists reqs0 n' n; unfold fold_right at 1; cancel.
-      rewrite interp_ghost; cancel.
-      rewrite <- (sepcon_emp (_ * _ * _)), sepcon_comm.
-      apply sepcon_derives; [|cancel].
-      apply andp_right; [apply prop_right; repeat split; auto; omega | apply derives_refl]. }
-    simpl; Intros reqs2 n1' n2'.
+  { forward_call (cprod, lock, sh, sh, lock_pred gsh2 buf ends len next ghosts).
+    { simpl.
+      Exists reqs0 times0 head0 tail0 n0 ns0; cancel. }
+    simpl; Intros reqs1 times1 head1 tail1 n1 ns1.
     forward.
-    Exists (reqs2, n1'); go_lower; unfold Znth; simpl; entailer'.
-    repeat rewrite interp_ghost.
-    rewrite sepcon_comm.
-    rewrite <- sepcon_assoc.
-    rewrite (sepcon_comm _ (ghost _ _ _ _)).
-    repeat rewrite <- sepcon_assoc.
-    do 7 rewrite sepcon_assoc.
-    eapply derives_trans; [apply sepcon_derives; [apply prop_and_same_derives, ghost_inj | apply derives_refl]|].
-    normalize.
-    assert (n2' = n).
-    { rewrite <- (Int.signed_repr n2'), <- (Int.signed_repr n); try omega; congruence. }
-    subst; entailer'; cancel. }
+    Exists (reqs1, times1, head1, tail1, n1, ns1); go_lower; unfold Znth; simpl.
+    apply andp_right; [apply prop_right; repeat split; auto |
+      apply andp_right; [apply prop_right; repeat split; auto | normalize; cancel]]. }
+  simpl; normalize.
   rewrite Int.signed_repr, Zlength_correct in HRE.
   forward.
-  { unfold MAX in *; apply prop_right; rewrite Zlength_correct; omega. }
+  unfold Znth; simpl.
+  forward.
+  forward.
+  unfold upd_Znth; repeat rewrite sublist.sublist_nil; simpl.
+  forward.
+  unfold Znth; simpl.
+  forward.
+  { apply prop_right.
+    replace (Z.of_nat tail0) with ((Z.of_nat head0 + Zlength reqs0) mod 10) by auto.
+    apply Z_mod_lt; omega. }
+  forward.
+  { repeat apply andp_right.
+    - go_lower; entailer'.
+    - go_lower; simpl.
+      apply prop_right.
+      rewrite andb_false_intro2; simpl; auto.
+    - go_lower; entailer'.
+    - apply TT_right. }
   forward.
   forward_call (ccon, sh).
   { simpl; cancel. }
-  assert (length reqs0 < 10)%nat by (rewrite Nat2Z.inj_lt; auto).
+  assert (length reqs0 < MAX)%nat by (rewrite Nat2Z.inj_lt; auto).
+  rewrite upd_rotate; auto.
+  replace ((Z.of_nat tail0 - Z.of_nat head0) mod Z.of_nat MAX) with (Zlength reqs0).
   rewrite upd_complete; auto.
-  unfold upd_Znth; repeat rewrite sublist.sublist_nil; simpl.
-  rewrite add_repr.
-  rewrite field_at_isptr, (field_at_isptr _ (tarray tint 1)), data_at_isptr; normalize.
-  forward_call (lock, sh, lock_pred gsh2 buf len next).
-  { simpl; unfold fold_right at 1; cancel.
-    Exists (reqs0 ++ [request]) n' n.
-    rewrite (data_at_isptr _ trequest); normalize.
-    destruct request; try contradiction; simpl.
-    repeat rewrite Zlength_correct; rewrite app_length; simpl.
-    eapply derives_trans; [|apply prop_and_same_derives'; unfold MAX; omega].
-    rewrite Nat2Z.inj_add; simpl; cancel.
-    repeat rewrite map_app; rewrite sepcon_app; simpl.
-    rewrite interp_ghost.
-    Exists data; unfold fold_right at 1; cancel.
-    entailer!; omega. }
+  unfold upd_Znth; simpl.
+  repeat rewrite sublist.sublist_nil.
+  repeat rewrite add_repr.
+  rewrite field_at_isptr, (field_at_isptr _ (tarray tint 1)), (field_at_isptr _ _ _ _ next),
+    (field_at_isptr _ trequest); normalize.
+  forward_call (lock, sh, lock_pred gsh2 buf ends len next ghosts).
+  { simpl.
+    Exists (reqs0 ++ [request]) (times0 ++ [n0]) head0 (Nat.modulo (tail0 + 1) MAX) (n0 + 1) ns0;
+      unfold fold_right at 1; cancel.
+    rewrite Zlength_app, Zlength_cons; simpl Z.succ; cancel.
+    unfold sem_mod; simpl sem_binarith.
+    unfold both_int; simpl force_val.
+    rewrite andb_false_intro2; [|simpl; auto].
+    simpl force_val.
+    rewrite mods_repr; try computable.
+    rewrite mod_Zmod, Nat2Z.inj_add; [cancel | omega].
+    rewrite <- (sepcon_emp (_ * _)), sepcon_comm.
+    match goal with H : _ /\ _ |- _ => destruct H as (? & ? & ?) end.
+    rewrite (sepcon_assoc (_ && _)); apply sepcon_derives.
+    { apply andp_right; auto; apply prop_right.
+      repeat split; auto; try omega.
+      - rewrite Forall_app; split.
+        + eapply Forall_impl; [|eauto].
+          intros ? (? & ?); split; auto; omega.
+        + constructor; auto.
+          repeat split; auto; try omega.
+          eapply Forall_impl; [|eauto]; intros ? (? & ?); auto.
+      - admit. (* Here's where we need to watch for overflow. *)
+      - eapply Forall_impl; [|eauto]; intros; simpl in *; omega.
+      - rewrite app_length; simpl; omega.
+      - repeat rewrite app_length; simpl; omega.
+      - apply SetoidList.SortA_app with (eqA := eq); auto.
+        intros ?? Hin Hn; inversion Hn; [|rewrite SetoidList.InA_nil in *; contradiction]; subst.
+        rewrite SetoidList.InA_alt in Hin; destruct Hin as (? & ? & Hin); subst.
+        match goal with H : Forall _ _ |- _ => rewrite Forall_forall in H; specialize (H _ Hin) end; omega.
+      - rewrite Z.add_assoc.
+        replace (Z.of_nat tail0) with ((Z.of_nat head0 + Zlength reqs0) mod 10) by auto.
+        rewrite Zplus_mod_idemp_l; auto. }
+      rewrite combine_app; auto; simpl.
+      repeat rewrite map_app; repeat rewrite sepcon_app; simpl.
+      Exists d; cancel.
+      { pose proof (Z_mod_lt (Z.of_nat head0 + Zlength reqs0) (Z.of_nat MAX)).
+        split; try omega.
+        transitivity (Z.of_nat MAX); simpl in *; [omega | computable]. } }
   { split; auto; split; [apply inv_precise | apply inv_positive]; auto. }
   forward.
-  Exists n; normalize; cancel.
-  { match goal with H : _ /\ _ |- _ => destruct H end.
-    pose proof Int.min_signed_neg.
-    rewrite Zlength_correct; split; try omega.
+  { cancel. }
+  { replace (Z.of_nat tail0) with ((Z.of_nat head0 + Zlength reqs0) mod 10) by auto.
+    rewrite Zminus_mod_idemp_l; auto.
+    rewrite Z.add_simpl_l, Zmod_small; auto; simpl.
+    rewrite Zlength_correct; omega. }
+  { apply length_complete; omega. }
+  { rewrite length_complete; [|omega].
+    replace (Z.of_nat tail0) with ((Z.of_nat head0 + Zlength reqs0) mod 10) by auto.
+    apply Z_mod_lt; omega. }
+  { pose proof Int.min_signed_neg; rewrite Zlength_correct; split; try omega.
+    match goal with H : _ /\ _ |- _ => destruct H as (? & ? & ?) end.
     transitivity (Z.of_nat MAX); [Omega0 | simpl; computable]. }
 Qed.
 
-Lemma all_ptrs : forall n reqs, fold_right sepcon emp (map Interp (map (fun r => Exp _ (fun data =>
-  Pred_list [Pred_prop (data < n); Data_at CompSpecs Tsh trequest (Vint (Int.repr data)) r])) reqs)) |--
+Lemma all_ptrs : forall reqs times, length times = length reqs ->
+  fold_right sepcon emp (map Interp (map (fun p => Exp val (fun d =>
+    Data_at _ Tsh trequest (d, Vint (Int.repr (fst p))) (snd p))) (combine times reqs))) |--
   !!(Forall isptr reqs).
 Proof.
-  induction reqs; simpl; entailer.
-  rewrite data_at_isptr.
-  eapply derives_trans; [apply sepcon_derives; [apply derives_refl | apply IHreqs]|].
+  induction reqs; simpl; intros; entailer.
+  destruct times; [discriminate | simpl].
+  Intro d; rewrite data_at_isptr.
   eapply derives_trans; [apply saturate_aux20|].
   { apply andp_left1, derives_refl. }
-  { apply derives_refl. }
+  { apply IHreqs; auto. }
   normalize.
 Qed.
 
-Lemma last_cons : forall {A} (d : A) l x, l <> [] -> last (x :: l) d = last l d.
+Lemma Znth_head : forall reqs head m d, (length reqs <= m)%nat -> (head < m)%nat ->
+  (length reqs > 0)%nat ->
+  Znth (Z.of_nat head) (rotate (complete m reqs) head m) d = Znth 0 reqs d.
+Proof.
+  intros; unfold rotate.
+  assert (Zlength (skipn (m - head) (complete m reqs)) = Z.of_nat head) as Hlen.
+  { rewrite Zlength_correct, skipn_length, length_complete; auto; Omega0. }
+  rewrite app_Znth2; rewrite Hlen; [|omega].
+  rewrite Zminus_diag.
+  rewrite <- (Nat2Z.id (m - head)), Znth_firstn; [|Omega0].
+  rewrite Znth_complete; auto.
+  rewrite Zlength_correct; omega.
+Qed.
+
+Opaque Nat.modulo.
+
+Lemma rotate_1 : forall v l n m, (n < m)%nat -> (length l < m)%nat ->
+  rotate (upd_Znth 0 (complete m (v :: l)) (Vint (Int.repr 0))) n m =
+  rotate (complete m l) (S n mod m) m.
 Proof.
   intros.
-  destruct l; auto.
-  contradiction H; auto.
+  unfold complete at 1; simpl.
+  unfold upd_Znth; simpl.
+  rewrite Zlength_cons; unfold sublist.sublist; simpl.
+  replace (Z.to_nat _) with (length (l ++ repeat (Vint (Int.repr 0)) (m - S (length l)))).
+  rewrite firstn_exact_length.
+  unfold rotate.
+  destruct (m - n)%nat eqn: Hminus; [omega | simpl].
+  destruct (eq_dec (S n) m).
+  - rewrite e, NPeano.Nat.mod_same; [|omega].
+    replace (m - 0)%nat with (length (complete m l)) by (rewrite length_complete; auto; omega).
+    rewrite skipn_exact_length, firstn_exact_length; simpl.
+    assert (n0 = O) by omega; subst; simpl.
+    unfold complete.
+    replace (S n - length l)%nat with (n - length l + 1)%nat by omega.
+    rewrite repeat_plus, <- app_assoc; auto.
+  - rewrite Nat.mod_small; [|omega].
+    assert (n0 = m - S n)%nat by omega; subst.
+    unfold complete.
+    replace (m - length l)%nat with (m - S (length l) + 1)%nat by omega.
+    rewrite repeat_plus; repeat rewrite app_assoc; simpl.
+    assert (m - S n <= Datatypes.length (l ++ repeat (Vint (Int.repr 0)) (m - S (Datatypes.length l))))%nat.
+    { rewrite app_length, repeat_length; omega. }
+    setoid_rewrite skipn_app1 at 2; auto; setoid_rewrite firstn_app1 at 2; auto.
+    rewrite <- app_assoc; auto.
+  - rewrite Zlength_correct; Omega0.
 Qed.
 
-Lemma nth_last : forall {A} (d : A) l, nth (length l - 1) l d = last l d.
+Lemma upd_Znth_length : forall {A} i (l : list A) x, 0 <= i < Z.of_nat (length l) ->
+  length (upd_Znth i l x) = length l.
 Proof.
-  induction l; auto.
-  simpl nth.
-  destruct (length l) eqn: Hlen.
-  { destruct l; simpl in *; [auto | omega]. }
-  rewrite last_cons; simpl in *; [|intro; subst; discriminate].
-  rewrite NPeano.Nat.sub_0_r in IHl; auto.
-Qed.
-
-Lemma Znth_last : forall {A} l (d : A), Znth (Zlength l - 1) l d = last l d.
-Proof.
-  intros; unfold Znth.
-  destruct (zlt (Zlength l - 1) 0).
-  - destruct l; auto.
-    rewrite Zlength_correct in *; simpl length in *.
-    rewrite Nat2Z.inj_succ in *; omega.
-  - rewrite Z2Nat.inj_sub; [|omega].
-    rewrite Zlength_correct, Nat2Z.id; simpl.
-    apply nth_last.
+  intros.
+  rewrite <- (Nat2Z.id (length _)), <- Zlength_correct.
+  rewrite upd_Znth_Zlength, Zlength_correct, Nat2Z.id; auto.
+  rewrite Zlength_correct; omega.
 Qed.
 
 Lemma body_remove : semax_body Vprog Gprog f_remove remove_spec.
 Proof.
   start_function.
-  forward_call (lock, sh, lock_pred gsh2 buf len next).
-  simpl; Intros reqs n1 n2.
+  forward_call (lock, sh, lock_pred gsh2 buf ends len next ghosts).
+  simpl; Intros reqs times head tail n ns.
   forward.
   unfold Znth; simpl.
-  forward_while (EX reqs : list val, EX n' : Z, PROP (n <= n' <= Int.max_signed /\ (length reqs <= MAX)%nat)
-   LOCAL (temp _len (Vint (Int.repr (Zlength reqs))); gvar _buf buf; 
-   gvar _length len; gvar _requests_lock lock; gvar _requests_producer cprod; gvar _requests_consumer ccon)
-   SEP (lock_inv sh lock (Interp (lock_pred gsh2 buf len next));
-        data_at Ews (tarray (tptr trequest) 10) (complete reqs) buf;
-        data_at Ews (tarray tint 1) [Vint (Int.repr (Zlength reqs))] len; emp;
-        data_at Ews (tarray tint 1) [Vint (Int.repr n')] next;
-        fold_right sepcon emp (map Interp (map (fun r => Exp Z (fun data =>
-          Pred_list [Pred_prop (data < n'); Data_at CompSpecs Tsh trequest (Vint (Int.repr data)) r])) reqs));
-        cond_var sh cprod; cond_var sh ccon;
-        ghost gsh1 tint (Vint (Int.repr n)) next; ghost gsh2 tint (Vint (Int.repr n)) next)).
-  { Exists reqs n1; entailer.
-    repeat rewrite interp_ghost.
-    rewrite sepcon_comm.
-    rewrite <- sepcon_assoc.
-    rewrite (sepcon_comm _ (ghost _ _ _ _)).
-    repeat rewrite <- sepcon_assoc.
-    do 6 rewrite sepcon_assoc.
-    eapply derives_trans; [apply sepcon_derives; [apply prop_and_same_derives, ghost_inj | apply derives_refl]|].
-    normalize.
-    assert (n2 = n).
-    { rewrite <- (Int.signed_repr n2), <- (Int.signed_repr n); try omega; congruence. }
-    subst; entailer'; cancel. }
-  { entailer. }
-  { forward_call (ccon, lock, sh, sh, lock_pred gsh2 buf len next).
-    { simpl; cancel.
-      Exists reqs0 n' n; unfold fold_right at 1; cancel.
-      rewrite interp_ghost; cancel.
-      rewrite <- (sepcon_emp (_ * _)), sepcon_comm.
-      apply sepcon_derives; [|cancel].
-      apply andp_right; [apply prop_right; repeat split; auto; try omega | apply derives_refl]. }
-    simpl; Intros reqs2 n1' n2'.
+  forward_while (EX reqs : list val, EX times : list Z, EX head : nat, EX tail : nat, EX n : Z, EX ns : list Z,
+   PROP ()
+   LOCAL (temp _len (Vint (Int.repr (Zlength reqs))); gvar _buf buf; gvar _ends ends; gvar _length len;
+          gvar _requests_lock lock; gvar _requests_producer cprod; gvar _requests_consumer ccon)
+   SEP (lock_inv sh lock (Interp (lock_pred gsh2 buf ends len next ghosts));
+        Interp (lock_pred' gsh2 buf ends len next ghosts reqs times head tail n ns);
+        cond_var sh cprod; cond_var sh ccon; ghost gsh1 tint (Vint (Int.repr t)) g)).
+  { Exists reqs times head tail n ns; go_lower.
+    apply andp_right; [apply prop_right; repeat split; auto |
+      apply andp_right; [apply prop_right; repeat split; auto | normalize; cancel]]. }
+  { go_lower; entailer'. }
+  { forward_call (ccon, lock, sh, sh, lock_pred gsh2 buf ends len next ghosts).
+    { simpl.
+      Exists reqs0 times0 head0 tail0 n0 ns0; cancel. }
+    simpl; Intros reqs1 times1 head1 tail1 n1 ns1.
     forward.
-    Exists (reqs2, n1'); go_lower; unfold Znth; simpl; entailer'.
-    repeat rewrite interp_ghost.
-    rewrite sepcon_comm.
-    rewrite <- sepcon_assoc.
-    rewrite (sepcon_comm _ (ghost _ _ _ _)).
-    repeat rewrite <- sepcon_assoc.
-    do 6 rewrite sepcon_assoc.
-    eapply derives_trans; [apply sepcon_derives; [apply prop_and_same_derives, ghost_inj | apply derives_refl]|].
-    normalize.
-    assert (n2' = n).
-    { rewrite <- (Int.signed_repr n2'), <- (Int.signed_repr n); try omega; congruence. }
-    subst; entailer'; cancel. }
+    Exists (reqs1, times1, head1, tail1, n1, ns1); go_lower; unfold Znth; simpl.
+    apply andp_right; [apply prop_right; repeat split; auto |
+      apply andp_right; [apply prop_right; repeat split; auto | normalize; cancel]]. }
+  simpl; normalize.
   assert (length reqs0 > 0)%nat.
   { rewrite Zlength_correct in *.
     destruct (length reqs0); [|omega].
     contradiction HRE; auto. }
-  assert (0 <= Zlength reqs0 - 1 < Z.of_nat MAX).
-  { rewrite Zlength_correct.
-    match goal with H : _ /\ _ |- _ => destruct H end; Omega0. }
+  match goal with H : _ /\ _ |- _ => destruct H as (? & ? & ?) end.
+  assert (0 <= Z.of_nat head0 < Z.of_nat MAX) by Omega0.
+  forward.
+  unfold Znth; simpl.
   forward.
   { go_lower; normalize.
-    rewrite Znth_complete; [|omega].
+    rewrite Znth_head; auto.
     do 4 rewrite sepcon_assoc; rewrite sepcon_comm.
-    repeat rewrite sepcon_assoc.
-    eapply derives_trans; [apply sepcon_derives; [apply prop_and_same_derives, all_ptrs | apply derives_refl]|].
+    rewrite map_app, sepcon_app.
+    repeat rewrite sepcon_assoc; rewrite sepcon_comm.
+    rewrite sepcon_assoc.
+    eapply derives_trans; [apply sepcon_derives; [apply prop_and_same_derives, all_ptrs; auto |
+      apply derives_refl]|].
     normalize; apply prop_right.
     apply Forall_Znth.
     { rewrite Zlength_correct; omega. }
@@ -488,46 +666,234 @@ Proof.
     destruct a; auto. }
   forward.
   forward.
+  { go_lower; normalize; simpl.
+    apply prop_right; rewrite andb_false_intro2; simpl; auto. }
+  forward.
   forward_call (cprod, sh).
   { simpl; cancel. }
-  rewrite field_at_isptr, (field_at_isptr _ (tarray tint 1)), data_at_isptr; normalize.
-  forward_call (lock, sh, lock_pred gsh2 buf len next).
+  rewrite upd_rotate; auto.
+  rewrite Zminus_diag, Zmod_0_l.
+  destruct reqs0; [contradiction HRE; auto|].
+  rewrite rotate_1; auto.
+  repeat rewrite Zlength_correct; simpl length.
+  repeat rewrite Nat2Z.inj_succ.
+  unfold upd_Znth; unfold sublist.sublist; simpl.
+  unfold sem_mod; simpl sem_binarith.
+  unfold both_int; simpl force_val.
+  rewrite andb_false_intro2; [|simpl; auto].
+  simpl force_val.
+  rewrite add_repr, mods_repr; try computable.
+  rewrite sub_repr.
+  unfold Z.succ; rewrite Z.add_simpl_r.
+  destruct times0; [discriminate | rewrite map_app, sepcon_app; simpl].
+  Intro d.
+  rewrite field_at_isptr, (field_at_isptr _ (tarray tint 1)), data_at_isptr,
+    (data_at_isptr _ trequest); normalize.
+  assert (i < length ghosts)%nat as Hlt by (rewrite <- nth_error_Some; intro X; rewrite X in *; discriminate).
+  replace (length ghosts) with (length ns0) in Hlt by auto.
+  forward_call (lock, sh, lock_pred gsh2 buf ends len next ghosts).
   { simpl.
-    assert (reqs0 <> []) as Hreqs by (destruct reqs0; [simpl in *; omega | discriminate]).
-    rewrite (app_removelast_last Vundef Hreqs) in *.
-    replace (Zlength _ - 1) with (Zlength (removelast reqs0)).
-    assert (length (removelast reqs0) < MAX)%nat.
-    { rewrite app_length in *; simpl in *; omega. }
-    rewrite remove_complete; auto.
-    unfold upd_Znth; simpl.
-    rewrite sublist.sublist_nil; simpl.
-    Exists (removelast reqs0) n' n'; unfold fold_right at 1; cancel.
-    repeat rewrite map_app; rewrite sepcon_app; simpl; cancel.
-    erewrite sepcon_assoc, ghost_join; eauto.
-    eapply derives_trans; [apply sepcon_derives; [apply derives_refl |
-      apply change_ghost with (v' := Vint (Int.repr n'))]|].
+    Exists reqs0 times0 (Nat.modulo (S head0) MAX) tail0 n0 (upd_Znth (Z.of_nat i) ns0 z); cancel.
+    rewrite <- Zlength_correct.
+    rewrite mod_Zmod, Nat2Z.inj_succ; simpl; [cancel | omega].
+    rewrite <- (sepcon_emp (_ * _)), sepcon_comm.
+    match goal with H : Forall _ (_ :: _) |- _ => inv H end.
+    rewrite (sepcon_assoc (_ && _)); apply sepcon_derives.
+    { apply andp_right; auto; apply prop_right.
+      match goal with H : Sorted _ _ |- _ => inv H end.
+      repeat split; auto; try omega.
+      - rewrite Forall_forall in *; intros ? Hin.
+        match goal with H : forall _, _ -> _ /\ _ |- _ => specialize (H _ Hin); destruct H; split; auto end.
+        apply Forall_upd_Znth; auto.
+        rewrite SetoidList.InfA_alt with (eqA := eq) in *; auto.
+        match goal with H : forall _, _ -> _ |- _ => apply H end.
+        rewrite SetoidList.InA_alt; eauto.
+        { constructor; repeat intro; omega. }
+        { repeat intro; omega. }
+      - apply Forall_upd_Znth; auto; omega.
+      - simpl in *; omega.
+      - rewrite upd_Znth_length; auto; Omega0.
+      - apply NPeano.Nat.mod_upper_bound; omega.
+      - rewrite Zlength_cons in *.
+        rewrite Zplus_mod_idemp_l; unfold Z.succ in *.
+        rewrite <- Zplus_assoc, (Zplus_comm 1); auto. }
+    exploit nth_ghost; eauto; intros (n2 & Hn2 & Heq); rewrite Heq.
+    rewrite sepcon_comm.
+    rewrite <- sepcon_assoc.
+    rewrite (sepcon_comm _ (ghost _ _ _ _)).
+    rewrite <- (sepcon_assoc _ (ghost _ _ _ _)), (sepcon_comm _ (ghost _ _ _ _)).
+    repeat rewrite <- sepcon_assoc.
+    do 4 rewrite sepcon_assoc.
+    eapply derives_trans; [apply sepcon_derives; [apply prop_and_same_derives, ghost_inj | apply derives_refl]|].
+    rewrite sepcon_andp_prop'; apply derives_extract_prop; intro.
+    assert (Int.min_signed <= n2 < n0).
+    { pose proof (nth_error_In _ _ Hn2) as Hin.
+      match goal with X : Forall _ _ |- _ => rewrite Forall_forall in X; specialize (X _ Hin); auto end. }
+    assert (n2 = t).
+    { rewrite <- (Int.signed_repr n2), <- (Int.signed_repr t); try omega; congruence. }
+    subst; erewrite ghost_join; eauto.
+    eapply derives_trans; [apply sepcon_derives; [apply change_ghost with (v' := Vint (Int.repr z)) |
+      apply derives_refl]|].
     erewrite <- ghost_join; eauto.
-    rewrite interp_ghost; cancel.
-    rewrite <- (sepcon_emp (_ * _ * _)), sepcon_comm.
-    apply sepcon_derives; [|cancel].
-    apply andp_right; [apply prop_right; repeat split; auto; omega | apply derives_refl].
-    { repeat rewrite Zlength_correct; rewrite app_length; simpl; Omega0. } }
+    repeat rewrite <- sepcon_assoc.
+    rewrite (sepcon_assoc (ghost _ _ _ _)), (sepcon_comm (ghost gsh2 _ _ _)).
+    repeat rewrite sepcon_assoc.
+    rewrite <- (sepcon_assoc (ghost gsh2 _ _ _)), (sepcon_comm (ghost gsh2 _ _ _)).
+    rewrite add_nth_ghost; auto.
+    subst Frame; instantiate (1 := [!!(t < z <= Int.max_signed) && emp; ghost _ tint _ _; cond_var _ _;
+      data_at _ trequest (_, _) _; cond_var _ _]).
+    simpl; rewrite map_app, sepcon_app; cancel.
+    normalize; apply andp_right; [apply prop_right | apply derives_refl].
+    pose proof (nth_error_In _ _ Hn2) as Hin.
+    match goal with X : _ /\ _ |- _ => destruct X as (? & X); rewrite Forall_forall in X;
+      specialize (X _ Hin); omega end. }
   { split; auto; split; [apply inv_precise | apply inv_positive]; auto. }
   forward.
-  Exists n'; normalize.
-  Exists (last reqs0 Vundef) x; normalize.
-  apply andp_right.
-  { apply prop_right; repeat split; auto.
-    rewrite Znth_complete; [|omega].
-    rewrite Znth_last; auto. }
-  cancel.
+  Exists z v d; normalize.
+  apply andp_right; [|cancel].
+  apply prop_right; repeat split; auto; try omega.
+  rewrite Znth_head; auto.
+  - split; try omega.
+    transitivity (Z.of_nat MAX); [omega | simpl; computable].
+  - rewrite length_complete; auto.
+  - rewrite length_complete; auto.
 Qed.
 
-Lemma body_f : semax_body Vprog Gprog f_producer producer_spec.
+Opaque lock_pred.
+
+Lemma upd_complete' : forall l x n, (length l < n)%nat -> 
+  upd_Znth (Zlength l) (map Vint (map Int.repr l) ++ repeat Vundef (n - length l)) (Vint (Int.repr x)) =
+  map Vint (map Int.repr (l ++ [x])) ++ repeat Vundef (n - length (l ++ [x])).
+Proof.
+  intros.
+  rewrite upd_Znth_app2.
+  repeat rewrite Zlength_correct; repeat rewrite map_length; repeat rewrite <- Zlength_correct.
+  rewrite Zminus_diag.
+  rewrite app_length; simpl plus.
+  destruct (n - length l)%nat eqn: Hminus; [omega|].
+  replace (n - (length l + 1))%nat with n0 by omega.
+  unfold upd_Znth, sublist.sublist; simpl.
+  rewrite Zlength_cons.
+  unfold Z.succ; rewrite Z.add_simpl_r.
+  rewrite Zlength_correct, Nat2Z.id, firstn_exact_length.
+  repeat rewrite map_app; rewrite <- app_assoc; auto.
+  { repeat rewrite Zlength_correct; repeat rewrite map_length; omega. }
+Qed.
+
+Lemma body_f : semax_body Vprog Gprog f_f f_spec.
 Proof.
   start_function.
+  rewrite (lock_inv_isptr _ lockt); normalize.
+  forward.
+  destruct lockt as [| | | | |lockt o]; try contradiction; simpl.
+  apply semax_seq' with (P' := PROP ( )
+   LOCAL (temp _l (Vptr lockt o); lvar _res (tarray tint 3) lvar0; 
+   gvar _buf buf; gvar _ends ends; gvar _length len; gvar _next next; gvar _requests_lock lock;
+   temp _arg (Vptr lockt o); gvar _requests_producer cprod; gvar _requests_consumer ccon)
+   SEP (data_at_ Tsh (tarray tint 3) lvar0; lock_inv sh lock (Interp (lock_pred gsh2 buf ends len next ghosts));
+   lock_inv sh (Vptr lockt o) (Interp (t_lock_pred sh cprod ccon lock (Vptr lockt o) buf ends len next ghosts gsh1 gsh2 g));
+   cond_var sh cprod; cond_var sh ccon; ghost gsh1 tint (Vint (Int.repr t)) g)).
+  { eapply semax_for_const_bound_const_init with (P := fun _ => [])
+      (Q := fun _ => [temp _l (Vptr lockt o); lvar _res (tarray tint 3) lvar0; 
+             gvar _buf buf; gvar _ends ends; gvar _length len; gvar _next next; gvar _requests_lock lock;
+             temp _arg (Vptr lockt o); gvar _requests_producer cprod; gvar _requests_consumer ccon])
+      (R := fun i => [data_at_ Tsh (tarray tint 3) lvar0;
+             lock_inv sh lock (Interp (lock_pred gsh2 buf ends len next ghosts));
+             lock_inv sh (Vptr lockt o) (Interp (t_lock_pred sh cprod ccon lock (Vptr lockt o) buf ends len next ghosts gsh1 gsh2 g));
+             cond_var sh cprod; cond_var sh ccon; ghost gsh1 tint (Vint (Int.repr t)) g]);
+    [reflexivity | try repable_signed | try repable_signed | reflexivity | try reflexivity; omega
+    | intro; unfold map at 1; auto 50 with closed
+    | cbv beta; simpl update_tycon
+    | intro; cbv beta; simpl update_tycon; try solve [entailer!]
+    | try apply semax_for_resolve_postcondition
+    | intro; cbv beta; simpl update_tycon; abbreviate_semax;
+      try (apply semax_extract_PROP; intro) ]; try computable.
+    { entailer!. }
+    { unfold normal_ret_assert; go_lower; entailer'. }
+    forward_call tt.
+    Intro x; destruct x as ((req, d0), t0); simpl.
+    forward_call (sh, lock, req, d0, t0, buf, ends, len, next, cprod, ccon, ghosts, gsh2).
+    go_lower; entailer'; cancel. }
+  subst MORE_COMMANDS; unfold abbreviate.
+  apply semax_seq' with (P' := PROP ( )
+   LOCAL (temp _l (Vptr lockt o); lvar _res (tarray tint 3) lvar0; gvar _buf buf; gvar _ends ends;
+   gvar _length len; gvar _next next; gvar _requests_lock lock; temp _arg (Vptr lockt o);
+   gvar _requests_producer cprod; gvar _requests_consumer ccon)
+   SEP ((EX d1 : Z, EX d2 : Z, EX d3 : Z, !! (d1 < d2 < d3) && data_at Tsh (tarray tint 3) [Vint (Int.repr d1);
+     Vint (Int.repr d2); Vint (Int.repr d3)] lvar0);
+   lock_inv sh lock (Interp (lock_pred gsh2 buf ends len next ghosts));
+   lock_inv sh (Vptr lockt o) (Interp (t_lock_pred sh cprod ccon lock (Vptr lockt o) buf ends len next ghosts gsh1 gsh2 g));
+   cond_var sh cprod; cond_var sh ccon;
+   EX n' : Z, !! (Int.min_signed <= n' <= Int.max_signed) && ghost gsh1 tint (Vint (Int.repr n')) g)).
+  { eapply semax_for_const_bound_const_init with (P := fun _ => [])
+      (Q := fun _ => [temp _l (Vptr lockt o); lvar _res (tarray tint 3) lvar0; 
+             gvar _buf buf; gvar _ends ends; gvar _length len; gvar _next next; gvar _requests_lock lock;
+             temp _arg (Vptr lockt o); gvar _requests_producer cprod; gvar _requests_consumer ccon])
+      (R := fun i => [EX n' : Z, EX ld : list Z, !! (Int.min_signed <= n' <= Int.max_signed /\
+             Zlength ld = i /\ Sorted Z.lt ld /\ Forall (fun z => Int.min_signed <= z <= n') ld) &&
+             data_at Tsh (tarray tint 3) (map Vint (map Int.repr ld) ++ repeat Vundef (3 - length ld)%nat) lvar0 *
+             ghost gsh1 tint (Vint (Int.repr n')) g;
+             lock_inv sh lock (Interp (lock_pred gsh2 buf ends len next ghosts));
+             lock_inv sh (Vptr lockt o) (Interp (t_lock_pred sh cprod ccon lock (Vptr lockt o) buf ends len next ghosts gsh1 gsh2 g));
+             cond_var sh cprod; cond_var sh ccon]);
+    [reflexivity | try repable_signed | try repable_signed | reflexivity | try reflexivity; omega
+    | intro; unfold map at 1; auto 50 with closed
+    | cbv beta; simpl update_tycon
+    | intro; cbv beta; simpl update_tycon; try solve [entailer!]
+    | try apply semax_for_resolve_postcondition
+    | intro; cbv beta; simpl update_tycon; abbreviate_semax;
+      try (apply semax_extract_PROP; intro) ]; try computable.
+    { entailer!.
+      Exists t ([] : list Z); simpl; entailer. }
+    { unfold normal_ret_assert; entailer!.
+      normalize.
+      destruct ld as [|d1]; [discriminate|].
+      destruct ld as [|d2]; [discriminate|].
+      destruct ld as [|d3]; [discriminate|].
+      destruct ld.
+      Exists n' d1 d2 d3.
+      inversion H3 as [|?? Hsort2 Hlt1]; inv Hlt1.
+      inversion Hsort2 as [|?? Hsort3 Hlt2]; inv Hlt2; normalize.
+      { repeat rewrite Zlength_cons in *.
+        rewrite Zlength_correct in *; omega. } }
+    Intros n1 ld; normalize.
+    forward_call (sh, n1, lock, buf, ends, len, next, cprod, ccon, ghosts, i, g, gsh1, gsh2).
+    Intro x; destruct x as ((t', req), d).
+    forward_call (req, d, t').
+    Intro v.
+    forward.
+    subst; simpl force_val.
+    rewrite upd_complete'; [|rewrite Zlength_correct in *; omega].
+    entailer.
+    Exists t' (ld ++ [t']); entailer!.
+    rewrite Zlength_app; simpl in *; split; [omega|].
+    split; auto; split.
+    - apply SetoidList.SortA_app with (eqA := eq); auto; intros.
+      rewrite SetoidList.InA_alt in *;
+        repeat match goal with H : exists _, _ |- _ => destruct H as (? & ? & ?); subst end.
+      match goal with H : In _ [_] |- _ => destruct H; [subst | contradiction] end.
+      match goal with H : In _ _, H' : Forall _ _ |- _ => rewrite Forall_forall in H';
+        specialize (H' _ H); omega end.
+    - rewrite Forall_app; split; [|constructor; auto; omega].
+      eapply Forall_impl; [|eauto]; intros; simpl in *; omega. }
+  Intros d1 d2 d3 n'.
+  forward_call (Vptr lockt o, sh, t_lock_pred sh cprod ccon lock (Vptr lockt o) buf ends len next ghosts gsh1 gsh2 g).
+  { simpl.
+    rewrite selflock_eq at 2; cancel.
+    Exists n'; rewrite interp_ghost; cancel.
+    rewrite sepcon_comm; apply sepcon_derives; [apply lock_inv_later | cancel]. }
+  { admit. }
+  eapply semax_pre; [|apply semax_return].
+  subst POSTCONDITION; unfold abbreviate.
+  go_lowerx; normalize.
+  unfold frame_ret_assert; simpl; entailer'.
+  Exists lvar0; normalize; cancel.
+Admitted.
 
-Qed.
+Axiom ghost_alloc : forall D P Q R t v p, ENTAIL D, PROPx P (LOCALx Q (SEPx R)) |--
+  PROPx P (LOCALx Q (SEPx (ghost Ews t v p :: R))).
+
+Transparent lock_pred.
 
 Lemma body_main:  semax_body Vprog Gprog f_main main_spec.
 Proof.
@@ -558,23 +924,43 @@ Proof.
   simpl init_data2pred'.
   rewrite <- (sepcon_emp (_ * _)).
   simple apply move_globfield_into_SEP.
+  rewrite sepcon_emp.
+  process_idstar.
+  simpl init_data2pred'.
+  rewrite <- (sepcon_emp (_ * _)).
+  simple apply move_globfield_into_SEP.
+  rewrite sepcon_emp.
+  process_idstar.
+  simpl init_data2pred'.
+  rewrite <- (sepcon_emp (_ * _)).
+  simple apply move_globfield_into_SEP.
+  rewrite sepcon_emp.
+  process_idstar.
+  simpl init_data2pred'.
+  rewrite <- (sepcon_emp (_ * _)).
+  simple apply move_globfield_into_SEP.
   change (globvars2pred nil) with (@emp (environ->mpred) _ _).
   repeat rewrite sepcon_emp.
   rewrite <- seq_assoc.
+  rename gvar7 into next, gvar6 into buf, gvar5 into cprod, gvar4 into ccon, gvar3 into ends, gvar2 into len,
+    gvar1 into lockt, gvar0 into lock.
   apply semax_seq' with (P' := PROP ( )
-    LOCAL (gvar _buf gvar4; gvar _requests_producer gvar3; gvar _requests_consumer gvar2;
-           gvar _length gvar1; gvar _requests_lock gvar0)
-    SEP (data_at Ews (tarray (tptr trequest) (Z.of_nat MAX)) (repeat (Vint (Int.repr 0)) MAX) gvar4;
-         data_at_ Ews tint gvar3; data_at_ Ews tint gvar2;
-         data_at_ Ews (tarray tint 1) gvar1;
-         data_at_ Ews (Tstruct 3%positive noattr) gvar0)).
+    LOCAL (gvar _next next; gvar _buf buf; gvar _requests_producer cprod; gvar _requests_consumer ccon;
+           gvar _ends ends; gvar _length len; gvar _thread_locks lockt; gvar _requests_lock lock)
+    SEP (data_at_ Ews (tarray tint 1) next;
+         data_at Ews (tarray (tptr (Tstruct 6%positive noattr)) 10) (repeat (Vint (Int.repr 0)) 10) buf;
+         data_at_ Ews tint cprod; data_at_ Ews tint ccon; data_at_ Ews (tarray tint 2) ends;
+         data_at_ Ews (tarray tint 1) len; data_at_ Ews (tarray (Tstruct 3%positive noattr) 3) lockt;
+         data_at_ Ews (Tstruct 3%positive noattr) lock)).
   { eapply semax_for_const_bound_const_init with (P := fun _ => [])
-      (Q := fun _ => [gvar _buf gvar4; gvar _requests_producer gvar3; gvar _requests_consumer gvar2; gvar _length gvar1; 
-                      gvar _requests_lock gvar0])
-      (R := fun i => [data_at Ews (tarray (tptr trequest) (Z.of_nat MAX))
-             (repeat (Vint (Int.repr 0)) (Z.to_nat i) ++ repeat Vundef (Z.to_nat (10 - i))) gvar4;
-             data_at_ Ews tint gvar3; data_at_ Ews tint gvar2;
-             data_at_ Ews (tarray tint 1) gvar1; data_at_ Ews tlock gvar0]);
+      (Q := fun _ => [gvar _next next; gvar _buf buf; gvar _requests_producer cprod; gvar _requests_consumer ccon;
+           gvar _ends ends; gvar _length len; gvar _thread_locks lockt; gvar _requests_lock lock])
+      (R := fun i => [data_at_ Ews (tarray tint 1) next;
+         data_at Ews (tarray (tptr (Tstruct 6%positive noattr)) 10)
+               (repeat (Vint (Int.repr 0)) (Z.to_nat i) ++ repeat Vundef (Z.to_nat (10 - i))) buf;
+         data_at_ Ews tint cprod; data_at_ Ews tint ccon; data_at_ Ews (tarray tint 2) ends;
+         data_at_ Ews (tarray tint 1) len; data_at_ Ews (tarray (Tstruct 3%positive noattr) 3) lockt;
+         data_at_ Ews (Tstruct 3%positive noattr) lock]);
     [reflexivity | try repable_signed | try repable_signed | reflexivity | try reflexivity; omega
     | intro; unfold map at 1; auto 50 with closed
     | cbv beta; simpl update_tycon
@@ -602,41 +988,157 @@ Proof.
     rewrite Z2Nat.inj_sub; [|omega].
     rewrite Hminus; simpl; omega. }
   forward.
-  forward_call (gvar0, Ews, lock_pred gvar4 gvar1).
+  forward.
+  forward.
+  forward.
+  unfold upd_Znth; repeat rewrite sublist.sublist_nil; simpl.
+  destruct split_Ews as (sh1 & sh2 & Hr1 & Hr2 & Hsh).
+  eapply semax_pre; [apply ghost_alloc with (t := tint)(v := Vint (Int.repr (-1)))(p := Vint (Int.repr 1))|].
+  eapply semax_pre; [apply ghost_alloc with (t := tint)(v := Vint (Int.repr (-1)))(p := Vint (Int.repr 2))|].
+  eapply semax_pre; [apply ghost_alloc with (t := tint)(v := Vint (Int.repr (-1)))(p := Vint (Int.repr 3))|].
+  set (ghosts := [Vint (Int.repr 1); Vint (Int.repr 2); Vint (Int.repr 3)]).
+  forward_call (lock, Ews, lock_pred sh2 buf ends len next ghosts).
   { unfold tlock, semax_conc._lock_t; cancel. }
-  rewrite (data_at_isptr _ (tarray _ _)), field_at_isptr; normalize.
-  forward_call (gvar0, Ews, lock_pred gvar4 gvar1).
+  rewrite (data_at_isptr _ (tarray _ _)), (field_at_isptr _ _ _ _ len), (field_at_isptr _ _ _ _ next);
+    normalize.
+  forward_call (lock, Ews, lock_pred sh2 buf ends len next ghosts).
   { simpl.
-    Exists ([] : list val); simpl; entailer!. }
+    Exists ([] : list val) ([] : list Z) O O 0 [-1; -1; -1]; unfold complete, rotate; simpl;
+      repeat rewrite interp_ghost; cancel; normalize.
+    apply andp_right; [|repeat rewrite <- (ghost_join _ _ _ _ _ _ Hsh); cancel].
+    apply prop_right; repeat split; auto; try omega; try computable.
+    - repeat (constructor; [computable|]); auto.
+    - unfold MAX; omega. }
   { split; auto; split.
     - apply inv_precise; auto.
     - apply inv_positive. }
-  forward_call (gvar3, Ews).
+  forward_call (cprod, Ews).
   { unfold tcond; cancel. }
-  forward_call (gvar2, Ews).
+  forward_call (ccon, Ews).
   { unfold tcond; cancel. }
-  destruct split_Ews as (sh1 & sh2 & ? & ? & Hsh).
-  get_global_function'' _consumer.
-  normalize.
-  apply extract_exists_pre; intros c_.
-  forward_call (c_, Vint (Int.repr 0), existT (fun ty => ty * (ty -> val -> Pred))%type
-   (val * val * share * val * val * val)%type ((gvar4, gvar1, sh1, gvar0, gvar3, gvar2),
-   fun (x : (val * val * share * val * val * val)) (_ : val) => let '(buf, len, sh, lock, cprod, ccon) := x in
-     Pred_list [Pred_prop (readable_share sh); Lock_inv sh lock (lock_pred buf len);
-                Cond_var _ sh cprod; Cond_var _ sh ccon])).
+  get_global_function'' _f; normalize.
+  apply extract_exists_pre; intros f_.
+  rewrite <- seq_assoc.
+  match goal with |-context[func_ptr' ?P] => set (spec := P) end.
+  destruct (split_readable_share _ Hr1) as (sh' & tsh2 & Hr' & ? & Hsh').
+  destruct (split_readable_share _ Hr') as (sh0 & tsh3 & ? & ? & Htsh).
+  (* break apart array into 3x data_at_ *)
+  rewrite data_at__isptr; normalize.
+  destruct lockt as [| | | | | b o]; try contradiction.
+  eapply semax_pre with (P' := PROP ( )
+   LOCAL (gvar _f f_; gvar _next next; gvar _buf buf; gvar _requests_producer cprod;
+   gvar _requests_consumer ccon; gvar _ends ends; gvar _length len; gvar _thread_locks (Vptr b o);
+   gvar _requests_lock lock)
+   SEP (func_ptr' spec f_; cond_var Ews ccon; cond_var Ews cprod;
+   lock_inv Ews lock (Interp (lock_pred sh2 buf ends len next ghosts));
+   ghost sh1 tint (Vint (Int.repr (-1))) (Vint (Int.repr 3));
+   ghost sh1 tint (Vint (Int.repr (-1))) (Vint (Int.repr 2));
+   ghost sh1 tint (Vint (Int.repr (-1))) (Vint (Int.repr 1));
+   data_at_ Ews tlock (Vptr b o); data_at_ Ews tlock (Vptr b (Int.add o (Int.repr 32)));
+   data_at_ Ews tlock (Vptr b (Int.add o (Int.repr 64))))).
+  { entailer!.
+    unfold data_at_, field_at_, field_at, at_offset; simpl.
+    rewrite int_add_repr_0_r.
+    rewrite data_at_rec_eq; simpl.
+    unfold array_pred, aggregate_pred.array_pred, at_offset, default_val, unfold_reptype, Znth; simpl.
+    normalize.
+    apply andp_right; [apply prop_right | apply derives_refl].
+    unfold field_compatible in *.
+    repeat match goal with H : _ /\ _ |- _ => destruct H end.
+    pose proof (Int.unsigned_range_2 o); simpl in *.
+    repeat rewrite <- (Int.repr_unsigned o), add_repr.
+    repeat rewrite Int.unsigned_repr; unfold Int.max_unsigned; try omega.
+    unfold align_attr, noattr; simpl.
+    repeat split; auto; simpl in *; try omega; apply Z.divide_add_r; auto.
+    - apply Zdivide_intro with (q := 16); auto.
+    - apply Zdivide_intro with (q := 8); auto. }
+  apply semax_seq' with (P' := PROP ( )
+    LOCAL (gvar _f f_; gvar _next next; gvar _buf buf; gvar _requests_producer cprod;
+           gvar _requests_consumer ccon;
+           gvar _ends ends; gvar _length len; gvar _thread_locks (Vptr b o); gvar _requests_lock lock)
+    SEP (func_ptr' spec f_; cond_var sh0 ccon; cond_var sh0 cprod;
+         lock_inv sh0 lock (Interp (lock_pred sh2 buf ends len next ghosts));
+         lock_inv sh1 (Vptr b o) (Interp (t_lock_pred sh2 cprod ccon lock
+           (Vptr b o) buf ends len next ghosts sh1 sh2 (Vint (Int.repr 1))));
+         lock_inv sh1 (Vptr b (Int.add o (Int.repr 32))) (Interp (t_lock_pred tsh2 cprod ccon lock
+           (Vptr b (Int.add o (Int.repr 32))) buf ends len next ghosts sh1 sh2 (Vint (Int.repr 2))));
+         lock_inv sh1 (Vptr b (Int.add o (Int.repr 64))) (Interp (t_lock_pred tsh3 cprod ccon lock
+           (Vptr b (Int.add o (Int.repr 64))) buf ends len next ghosts sh1 sh2 (Vint (Int.repr 3)))))).
+  { eapply semax_for_const_bound_const_init with (P := fun _ => [])
+      (Q := fun _ => [gvar _f f_; gvar _next next; gvar _buf buf; gvar _requests_producer cprod; gvar _requests_consumer ccon;
+           gvar _ends ends; gvar _length len; gvar _thread_locks (Vptr b o); gvar _requests_lock lock])
+      (R := fun i => let s1 := nth (Z.to_nat i) [Ews; sh1; sh'] sh0 in
+        [func_ptr' spec f_; cond_var s1 ccon; cond_var s1 cprod;
+         lock_inv s1 lock (Interp (lock_pred sh2 buf ends len next ghosts))] ++
+         firstn (Z.to_nat i) [lock_inv sh1 (Vptr b o) (Interp (t_lock_pred sh2 cprod ccon lock
+           (Vptr b o) buf ends len next ghosts sh1 sh2 (Vint (Int.repr 1))));
+         lock_inv sh1 (Vptr b (Int.add o (Int.repr 32))) (Interp (t_lock_pred tsh2 cprod ccon lock
+           (Vptr b (Int.add o (Int.repr 32))) buf ends len next ghosts sh1 sh2 (Vint (Int.repr 2))));
+         lock_inv sh1 (Vptr b (Int.add o (Int.repr 64))) (Interp (t_lock_pred tsh3 cprod ccon lock
+           (Vptr b (Int.add o (Int.repr 64))) buf ends len next ghosts sh1 sh2 (Vint (Int.repr 3))))] ++
+         skipn (Z.to_nat i) (map (fun i => ghost sh1 tint (Vint (Int.repr (-1))) (Vint (Int.repr i))) [1; 2; 3]) ++
+         skipn (Z.to_nat i) [data_at_ Ews tlock (Vptr b o);
+                             data_at_ Ews tlock (Vptr b (Int.add o (Int.repr 32)));
+                             data_at_ Ews tlock (Vptr b (Int.add o (Int.repr 64)))]);
+    [reflexivity | try repable_signed | try repable_signed | reflexivity | try reflexivity; omega
+    | intro; unfold map at 1; auto 50 with closed
+    | cbv beta; simpl update_tycon
+    | intro; cbv beta; simpl update_tycon; try solve [entailer!]
+    | try apply semax_for_resolve_postcondition
+    | intro; cbv beta; simpl update_tycon; abbreviate_semax;
+      try (apply semax_extract_PROP; intro) ]; try computable.
+    { go_lower; simpl.
+      apply andp_right; [apply prop_right; auto|].
+      apply andp_right; [apply prop_right; repeat split; auto | cancel]. }
+    { unfold normal_ret_assert; entailer!. }
+    destruct (eq_dec i 0); [|destruct (eq_dec i 1); [|assert (i = 2) by omega]]; subst; simpl.
+    - eapply semax_seq'.
+      let Frame := fresh "Frame" in evar (Frame: list (mpred));
+      eapply (semax_call_id00_wow (Vptr b o, Ews, t_lock_pred sh2 cprod ccon lock (Vptr b o) buf ends len next ghosts sh1 sh2
+        (Vint (Int.repr 1))) Frame);
+ [ check_function_name | lookup_spec_and_change_compspecs CompSpecs
+ | find_spec_in_globals | check_result_type | check_parameter_types
+ | check_prove_local2ptree
+ | (*check_typecheck*)
+ | check_funspec_precondition
+ | check_prove_local2ptree
+ | check_cast_params | reflexivity
+ | Forall_pTree_from_elements
+ | Forall_pTree_from_elements
+ | (*unfold fold_right at 1 2; cancel*)
+ | cbv beta iota; 
+    repeat rewrite exp_uncurry;
+    try rewrite no_post_exists0; 
+    first [reflexivity | extensionality; simpl; reflexivity]
+ | unify_postcondition_exps
+ | unfold fold_right_and; repeat rewrite and_True; auto
+ ].
+(*
+forward_call (Vptr b o, Ews, t_lock_pred sh2 cprod ccon lock (Vptr b o) buf ends len next ghosts sh1 sh2
+        (Vint (Int.repr 1))).
+      forward_call (f_, Vptr b o, existT (fun ty => ty * (ty -> val -> Pred))%type
+   (share * Z * val * val * val * val * val * val * val * val * list val * nat * val * share * share)%type
+   ((sh2, Vint (Int.repr (-1)), lock, buf, ends, len, next, Vptr b o, cprod, ccon, ghosts, 0, Vint (Int.repr 1), sh1, sh2),
+   fun (x : (share * Z * val * val * val * val * val * val * val * val * list val * nat * val * share * share)) (_ : val) =>
+   let '(sh, t, lock, buf, ends, len, next, lockt, cprod, ccon, ghosts, i, g, gsh1, gsh2) := x in
+     Pred_list [Pred_prop (readable_share sh /\ Int.min_signed <= t <= Int.max_signed /\
+                           sepalg.join gsh1 gsh2 Ews /\ nth_error ghosts i = Some g);
+       Lock_inv sh lock (lock_pred gsh2 buf ends len next ghosts);
+       Lock_inv sh lockt (t_lock_pred sh cprod ccon lock lockt buf ends len next ghosts gsh1 gsh2 g);
+       Cond_var _ sh cprod; Cond_var _ sh ccon; Ghost gsh1 tint (Vint (Int.repr t)) g])).
   { simpl; entailer.
     Exists _arg; entailer.
     Exists (fun x : val * val * share * val * val * val => let '(buf, len, sh, lock, cprod, ccon) := x in
       [(_buf, buf); (_length, len); (_requests_lock, lock); (_requests_producer, cprod);
        (_requests_consumer, ccon)]); entailer.
-    subst Frame; instantiate (1 := [cond_var sh2 gvar2; cond_var sh2 gvar3;
-      lock_inv sh2 gvar0 (Interp (lock_pred gvar4 gvar1))]).
+    subst Frame; instantiate (1 := [cond_var sh2 len; cond_var sh2 ends;
+      lock_inv sh2 lock (Interp (lock_pred ccon lockt))]).
     evar (body : funspec); replace (WITH _ : _ PRE [_] _ POST [_] _) with body.
     repeat rewrite sepcon_assoc; apply sepcon_derives; subst body; [apply derives_refl|].
     simpl.
-    erewrite <- (sepcon_assoc (cond_var sh1 gvar2)), cond_var_join; eauto; cancel.
+    erewrite <- (sepcon_assoc (cond_var sh1 len)), cond_var_join; eauto; cancel.
     repeat rewrite sepcon_assoc.
-    erewrite <- (sepcon_assoc (cond_var sh1 gvar3)), cond_var_join; eauto; cancel.
+    erewrite <- (sepcon_assoc (cond_var sh1 ends)), cond_var_join; eauto; cancel.
     erewrite lock_inv_join; eauto; cancel.
     subst body; f_equal.
     extensionality.
@@ -652,30 +1154,30 @@ Proof.
     - eapply cond_var_almost_empty; eauto.
     - eapply cond_var_almost_empty; eauto.
     - eapply emp_almost_empty; eauto. }
-  forward_call (gvar0, sh2, lock_pred gvar4 gvar1).
+  forward_call (lock, sh2, lock_pred ccon lockt).
   simpl.
   Intro reqs; normalize.
   forward.
   unfold Znth; simpl.
   forward_while (EX reqs : list val, PROP (Forall isptr reqs; (length reqs <= MAX)%nat)
-   LOCAL (temp _len (Vint (Int.repr (Zlength reqs))); gvar _consumer c_; gvar _buf gvar4; gvar _requests_producer gvar3;
-   gvar _requests_consumer gvar2; gvar _length gvar1; gvar _requests_lock gvar0)
-   SEP (data_at Ews (tarray (tptr trequest) (Z.of_nat MAX)) (complete reqs) gvar4;
-   data_at Ews (tarray tint 1) [Vint (Int.repr (Zlength reqs))] gvar1;
+   LOCAL (temp _len (Vint (Int.repr (Zlength reqs))); gvar _consumer c_; gvar _buf ccon; gvar _requests_producer ends;
+   gvar _requests_consumer len; gvar _length lockt; gvar _requests_lock lock)
+   SEP (data_at Ews (tarray (tptr trequest) (Z.of_nat MAX)) (complete reqs) ccon;
+   data_at Ews (tarray tint 1) [Vint (Int.repr (Zlength reqs))] lockt;
    fold_right sepcon emp
      (map Interp (map (fun r : val => Exp Z (fun data : Z => Data_at CompSpecs Tsh trequest (Vint (Int.repr data)) r)) reqs));
-   lock_inv sh2 gvar0 (Interp (lock_pred gvar4 gvar1));
-   cond_var sh2 gvar2; cond_var sh2 gvar3)).
+   lock_inv sh2 lock (Interp (lock_pred ccon lockt));
+   cond_var sh2 len; cond_var sh2 ends)).
   { Exists reqs; entailer!. }
   { entailer. }
   { (* loop body *)
-    forward_call (gvar3, gvar0, sh2, sh2, lock_pred gvar4 gvar1).
+    forward_call (ends, lock, sh2, sh2, lock_pred ccon lockt).
     { simpl; cancel.
       Exists reqs0; unfold fold_right at 1; cancel; entailer!. }
     simpl; Intro reqs'; normalize.
     forward.
     Exists reqs'; entailer!. }
-  forward_call (gvar0, sh2, lock_pred gvar4 gvar1).
+  forward_call (lock, sh2, lock_pred ccon lockt).
   { simpl; Exists reqs0; cancel.
     unfold fold_right at 1; entailer!. }
   { split; auto; split; [apply inv_precise | apply inv_positive]; auto. }
@@ -684,7 +1186,7 @@ Proof.
   normalize.
   apply extract_exists_pre; intros p_.
   forward_call (p_, Vint (Int.repr 0), existT (fun ty => ty * (ty -> val -> Pred))%type
-   (val * val * share * val * val * val)%type ((gvar4, gvar1, sh2', gvar0, gvar3, gvar2),
+   (val * val * share * val * val * val)%type ((ccon, lockt, sh2', lock, ends, len),
    fun (x : (val * val * share * val * val * val)) (_ : val) => let '(buf, len, sh, lock, cprod, ccon) := x in
      Pred_list [Pred_prop (readable_share sh); Lock_inv sh lock (lock_pred buf len);
                 Cond_var _ sh cprod; Cond_var _ sh ccon])).
@@ -693,14 +1195,14 @@ Proof.
     Exists (fun x : val * val * share * val * val * val => let '(buf, len, sh, lock, cprod, ccon) := x in
       [(_buf, buf); (_length, len); (_requests_lock, lock); (_requests_producer, cprod);
        (_requests_consumer, ccon)]); entailer.
-    subst Frame; instantiate (1 := [cond_var sh3 gvar2; cond_var sh3 gvar3;
-      lock_inv sh3 gvar0 (Interp (lock_pred gvar4 gvar1))]).
+    subst Frame; instantiate (1 := [cond_var sh3 len; cond_var sh3 ends;
+      lock_inv sh3 lock (Interp (lock_pred ccon lockt))]).
     evar (body : funspec); replace (WITH _ : _ PRE [_] _ POST [_] _) with body.
     repeat rewrite sepcon_assoc; apply sepcon_derives; subst body; [apply derives_refl|].
     simpl.
-    erewrite <- (sepcon_assoc (cond_var sh2' gvar2)), cond_var_join; eauto; cancel.
+    erewrite <- (sepcon_assoc (cond_var sh2' len)), cond_var_join; eauto; cancel.
     repeat rewrite sepcon_assoc.
-    erewrite <- (sepcon_assoc (cond_var sh2' gvar3)), cond_var_join; eauto; cancel.
+    erewrite <- (sepcon_assoc (cond_var sh2' ends)), cond_var_join; eauto; cancel.
     erewrite lock_inv_join; eauto; cancel.
     subst body; f_equal.
     extensionality.
@@ -720,8 +1222,8 @@ Proof.
   apply semax_seq' with (P' := PROP () LOCAL () SEP (FF)).
   { match goal with |- semax _ ?P _ _ => eapply semax_loop with (Q' := P) end;
       forward; entailer!. }
-  forward.
-Qed.
+  forward.*)
+Admitted.
 
 Definition extlink := ext_link_prog prog.
 
@@ -747,18 +1249,24 @@ semax_func_cons_ext.
 { admit. }
 semax_func_cons_ext.
 { admit. }
+semax_func_cons_ext.
+{ admit. }
+semax_func_cons_ext.
+{ admit. }
+semax_func_cons_ext.
+{ admit. }
+semax_func_cons_ext.
+{ admit. }
 eapply semax_func_cons_ext; try reflexivity.
 { admit. }
 { admit. }
 eapply semax_func_cons_ext; try reflexivity.
 { admit. }
 { admit. }
-semax_func_cons body_process.
 semax_func_cons body_get_request.
 semax_func_cons body_process_request.
 semax_func_cons body_add.
 semax_func_cons body_remove.
-semax_func_cons body_producer.
-semax_func_cons body_consumer.
+semax_func_cons body_f.
 semax_func_cons body_main.
 Admitted.
